src/prop/Single.v
@@ -48,6 +48,171 @@ Module SConfiguration.
   .
   Hint Constructors step.
 
+  Inductive steps:
+    forall (es: list ThreadEvent.t) (tid: Ident.t) (c1 c2:Configuration.t), Prop :=
+  | steps_nil
+      tid c1
+    :
+      steps [] tid c1 c1
+  | steps_cons
+      ehd etl tid c1 c2 c3
+      (STEP: step ehd tid c1 c2)
+      (STEPS: steps etl tid c2 c3)
+    :
+      steps (ehd :: etl) tid c1 c3
+  .
+  Hint Constructors steps.
+
+  (* Inductive steps: *)
+  (*   forall (es: list ThreadEvent.t) (tid: Ident.t) (c1 c2:Configuration.t), Prop := *)
+  (* | steps_base *)
+  (*     tid e c1 c2 *)
+  (*     (STEP: step e tid c1 c2) *)
+  (*   : *)
+  (*     steps [e] tid c1 c2 *)
+  (* | steps_cons *)
+  (*     ehd etl tid c1 c2 c3 *)
+  (*     (STEP: step ehd tid c1 c2) *)
+  (*     (STEPS: steps etl tid c2 c3) *)
+  (*   : *)
+  (*     steps (ehd :: etl) tid c1 c3 *)
+  (* . *)
+  (* Hint Constructors steps. *)
+
+  Lemma steps_trans es0 es1 tid c0 c1 c2
+        (STEPS0: steps es0 tid c0 c1)
+        (STEPS1: steps es1 tid c1 c2)
+    :
+      steps (es0 ++ es1) tid c0 c2.
+  Proof.
+    ginduction STEPS0; eauto.
+    { i. ss. econs; eauto. }
+  Qed.
+
+  Lemma steps_split es0 es1 tid c0 c2
+        (STEPS: steps (es0 ++ es1) tid c0 c2)
+    :
+      exists c1,
+        (<<STEPS0: steps es0 tid c0 c1>>) /\
+        (<<STEPS1: steps es1 tid c1 c2>>).
+  Proof.
+    ginduction es0; eauto. i. ss. inv STEPS.
+    exploit IHes0; eauto. i. des.
+    esplits; eauto.
+  Qed.
+
+  Inductive reservation_only_step:
+    forall (tid:Ident.t) (c1 c2:Configuration.t), Prop :=
+  | reservation_only_step_intro
+      tid c1 lang st1 lc1 e2 st4 lc4 sc4 memory4
+      (TID: IdentMap.find tid c1.(Configuration.threads) = Some (existT _ lang st1, lc1))
+      (CANCELS: rtc (@Thread.cancel_step _) (Thread.mk _ st1 lc1 c1.(Configuration.sc) c1.(Configuration.memory)) e2)
+      (RESERVES: rtc (@Thread.reserve_step _) e2 (Thread.mk _ st4 lc4 sc4 memory4))
+      (CONSISTENT: Thread.consistent (Thread.mk _ st4 lc4 sc4 memory4)):
+      reservation_only_step tid c1 (Configuration.mk (IdentMap.add tid (existT _ _ st4, lc4) c1.(Configuration.threads)) sc4 memory4)
+  .
+  Hint Constructors reservation_only_step.
+
+  Lemma reservation_only_step_step tid c1 c2
+        (STEP: reservation_only_step tid c1 c2)
+    :
+      step ThreadEvent.silent tid c1 c2.
+  Proof.
+    inv STEP. econs; eauto. econs 1.
+  Qed.
+
+  Lemma reservation_only_step_trans tid c1 c2 c3
+        (STEP1: reservation_only_step tid c1 c2)
+        (STEP2: reservation_only_step tid c2 c3)
+    :
+      reservation_only_step tid c1 c3.
+  Proof.
+    inv STEP1. inv STEP2. ss.
+    erewrite IdentMap.gss in TID0. dep_clarify. dep_clarify.
+    assert (STEPS: rtc
+                     (@Thread.reserve_step _ \2/ @Thread.cancel_step _)
+                     (Thread.mk _ st1 lc1 c1.(Configuration.sc) c1.(Configuration.memory))
+                     (Thread.mk _ st2 lc2 sc0 memory0)).
+    { etrans.
+      { eapply rtc_implies; try apply CANCELS; eauto. }
+      etrans.
+      { eapply rtc_implies; try apply RESERVES; eauto. }
+      etrans.
+      { eapply rtc_implies; try apply CANCELS0; eauto. }
+      { eapply rtc_implies; try apply RESERVES0; eauto. }
+    }
+    eapply rtc_implies with (R2:=tau (@pred_step (ThreadEvent.is_reserve \1/ ThreadEvent.is_cancel) _)) in STEPS; cycle 1.
+    { clear. i. des.
+      { inv H. econs; eauto.
+        { econs; eauto.
+          { econs; eauto. }
+          { ss; auto. }
+        }
+        { ss. }
+      }
+      { inv H. econs; eauto.
+        { econs; eauto.
+          { econs; eauto. }
+          { ss; auto. }
+        }
+        { ss. }
+      }
+    }
+    hexploit steps_not_reserves_reserves; try apply STEPS. i. des.
+    erewrite IdentMap.add_add_eq. econs.
+    { eauto. }
+    { eapply rtc_implies; try apply STEPS1.
+      clear. i. inv H. inv TSTEP. des; ss. inv STEP.
+      unfold ThreadEvent.is_cancel in *. des_ifs. econs; eauto. }
+    { eapply STEPS2. }
+    { auto. }
+  Qed.
+
+  Lemma reserve_reservation_only_step e tid c1 c2
+        (STEP: step e tid c1 c2)
+        (RESERVE: ThreadEvent.is_reserve e)
+    :
+      reservation_only_step tid c1 c2.
+  Proof.
+    inv STEP. inv STEP0; ss. econs.
+    { eauto. }
+    { eauto. }
+    { unfold ThreadEvent.is_reserve in *. des_ifs. econs 2.
+      { econs; eauto. }
+      { eapply RESERVES. }
+    }
+    { eapply CONSISTENT. ii. clarify. }
+  Qed.
+
+  Lemma cancel_reservation_only_step e tid c1 c2
+        (STEP: step e tid c1 c2)
+        (CANCEL: ThreadEvent.is_cancel e)
+    :
+      reservation_only_step tid c1 c2.
+  Proof.
+    inv STEP. inv STEP0; ss. econs.
+    { eauto. }
+    { unfold ThreadEvent.is_cancel in *. des_ifs. etrans.
+      { eauto. }
+      { econs 2; [|refl]. econs; eauto. }
+    }
+    { eauto. }
+    { eapply CONSISTENT. ii. clarify. }
+  Qed.
+
+  Lemma reservation_event_reservation_only_step e tid c1 c2
+        (STEP: step e tid c1 c2)
+        (RESERVATION: ~ ThreadEvent.is_normal e)
+    :
+      reservation_only_step tid c1 c2.
+  Proof.
+    unfold ThreadEvent.is_normal in *. apply not_and_or in RESERVATION. des.
+    { apply NNPP in RESERVATION.
+      eapply reserve_reservation_only_step; eauto. }
+    { apply NNPP in RESERVATION.
+      eapply cancel_reservation_only_step; eauto. }
+  Qed.
+
   Inductive machine_step: forall (e:MachineEvent.t) (tid:Ident.t) (c1 c2:Configuration.t), Prop :=
   | machine_step_intro
       e tid c1 c2
@@ -165,6 +330,19 @@ Module SConfiguration.
       splits; eauto; etrans; eauto.
   Qed.
 
+  Lemma silent_steps_tau_machine_steps es tid c1 c2
+        (STEPS: steps es tid c1 c2)
+        (SILENT: List.Forall (fun e => ThreadEvent.get_machine_event e = MachineEvent.silent) es)
+    :
+      rtc tau_machine_step c1 c2.
+  Proof.
+    ginduction es; i.
+    { inv STEPS. eauto. }
+    { inv STEPS. inv SILENT. exploit IHes; eauto.
+      i. econs 2; eauto. econs; eauto.
+      rewrite <- H1. econs; eauto. }
+  Qed.
+
   Lemma step_mixed_step e tid c1 c2
         (STEP: step e tid c1 c2)
     :
@@ -181,49 +359,210 @@ Module SConfiguration.
   Lemma mixed_step_step e tid c1 c2
         (STEP: mixed_step e tid c1 c2)
     :
-      exists e',
-        (<<STEP: step e' tid c1 c2>>) /\
-        __guard__(e' = e \/ e' = ThreadEvent.silent /\ (<<RESERVE: is_reserve e>> \/ <<CANCEL: is_cancel e>>)).
+      (<<STEP: step e tid c1 c2>>) \/
+      ((<<STEP: reservation_only_step tid c1 c2>>) /\
+       (<<RESERVATION: ~ ThreadEvent.is_normal e>>)).
   Proof.
-    inv STEP. exploit reorder_reserves_opt_step_cancels.
+    inv STEP.
+    exploit reorder_reserves_opt_step_cancels.
     { eapply CANCELS. }
     { eauto. }
     { eapply RESERVES. }
-    i. des. esplits.
-    { econs.
+    i. des.
+    { left. econs.
       { eauto. }
       { eapply STEPS1. }
       { eapply STEP2. }
       { eapply STEPS3. }
-      { ii. eapply CONSISTENT; eauto. ii.
-        subst. unguard. des; ss. }
+      { eauto. }
     }
-    { eauto. }
+    { right. splits; auto. econs.
+      { eauto. }
+      { eapply STEPS1. }
+      { eapply STEPS3. }
+      { eapply CONSISTENT; eauto. ii. clarify.
+        unfold ThreadEvent.is_normal in *. eauto. }
+    }
   Qed.
 
-  Lemma multi_step_machine_step e tid c1 c3
-        (STEP: Configuration.step e tid c1 c3)
+  Lemma merge_reservation_only_step_step e tid c1 c2 c3
+        (STEP0: reservation_only_step tid c1 c2)
+        (STEP1: step e tid c2 c3)
+    :
+      (<<STEP: step e tid c1 c3>>) \/
+      ((<<STEP: reservation_only_step tid c1 c3>>) /\
+       (<<RESERVATION: ~ ThreadEvent.is_normal e>>)).
+  Proof.
+    inv STEP0. inv STEP1. ss.
+    erewrite IdentMap.gss in TID0. dep_clarify. dep_clarify.
+    erewrite IdentMap.add_add_eq.
+    exploit mixed_step_step.
+    { econs.
+      { eapply TID. }
+      { etrans.
+        { eapply rtc_implies; try apply CANCELS. eauto. }
+        etrans.
+        { eapply rtc_implies; try apply RESERVES. eauto. }
+        { eapply rtc_implies; try apply CANCELS0. eauto. }
+      }
+      { eauto. }
+      { eapply rtc_implies; try apply RESERVES0. eauto. }
+      { eauto. }
+    }
+    i. des; eauto.
+  Qed.
+
+  Lemma merge_step_reservation_only_step e tid c1 c2 c3
+        (STEP0: step e tid c1 c2)
+        (STEP1: reservation_only_step tid c2 c3)
+    :
+      (<<STEP: step e tid c1 c3>>) \/
+      ((<<STEP: reservation_only_step tid c1 c3>>) /\
+       (<<RESERVATION: ~ ThreadEvent.is_normal e>>)).
+  Proof.
+    inv STEP0. inv STEP1. ss.
+    erewrite IdentMap.gss in TID0. dep_clarify. dep_clarify.
+    erewrite IdentMap.add_add_eq.
+    exploit mixed_step_step.
+    { econs.
+      { eapply TID. }
+      { eapply rtc_implies; try apply CANCELS. eauto. }
+      { eauto. }
+      { etrans.
+        { eapply rtc_implies; try apply RESERVES. eauto. }
+        etrans.
+        { eapply rtc_implies; try apply CANCELS0. eauto. }
+        { eapply rtc_implies; try apply RESERVES0. eauto. }
+      }
+      { eauto. }
+    }
+    i. des; eauto.
+  Qed.
+
+  Lemma list_filter_idempotent A P (l: list A)
+    :
+      List.filter P (List.filter P l) = List.filter P l.
+  Proof.
+    induction l; eauto. ss. des_ifs. ss. des_ifs. f_equal; auto.
+  Qed.
+
+  Lemma list_filter_app A P (l0 l1: list A)
+    :
+      List.filter P (l0 ++ l1) = (List.filter P l0) ++ (List.filter P l1) .
+  Proof.
+    induction l0; eauto. ss. des_ifs. ss. f_equal; auto.
+  Qed.
+
+  Lemma steps_filtering es tid c1 c2
+        (STEPS: steps es tid c1 c2)
+    :
+      (<<STEPS: steps (List.filter ThreadEvent.is_normal_dec es) tid c1 c2>>) \/
+      ((<<STEP: reservation_only_step tid c1 c2>>) /\
+       (<<RESERVATION: List.filter ThreadEvent.is_normal_dec es = []>>)).
+  Proof.
+    ginduction es; eauto. i. inv STEPS. ss. unfold proj_sumbool in *. des_ifs.
+    { exploit IHes; eauto. i. des.
+      { left. econs; eauto. }
+      { rewrite RESERVATION in *. left. econs 2; [|econs 1].
+        exploit merge_step_reservation_only_step; eauto. i. des; ss. }
+    }
+    { eapply reservation_event_reservation_only_step in STEP; auto.
+      exploit IHes; eauto. i. des.
+      { inv STEPS.
+        { right. splits; eauto. }
+        { left. exploit merge_reservation_only_step_step; eauto. i. des.
+          { econs; eauto. }
+          { exfalso.
+            hexploit
+              (proj1 (List.filter_In
+                        (fun e => if ThreadEvent.is_normal_dec e then true else false) ehd es)).
+            { rewrite <- H0. ss. auto. }
+            i. des. des_ifs.
+          }
+        }
+      }
+      { rewrite RESERVATION in *. right. splits; auto.
+        eapply reservation_only_step_trans; eauto. }
+    }
+  Qed.
+
+  Lemma merge_reservation_only_step_steps es tid c1 c2 c3
+        (STEP0: reservation_only_step tid c1 c2)
+        (STEP1: steps es tid c2 c3)
+    :
+      (<<STEPS: steps (List.filter ThreadEvent.is_normal_dec es) tid c1 c3>>) \/
+      ((<<STEP: reservation_only_step tid c1 c3>>) /\
+       (<<RESERVATION: List.filter ThreadEvent.is_normal_dec es = []>>)).
+  Proof.
+    hexploit steps_filtering; try apply STEP1. i. des.
+    { inv STEPS.
+      { right. splits; auto. }
+      { left. exploit merge_reservation_only_step_step; eauto. i. des.
+        { econs; eauto. }
+        { exfalso.
+          hexploit
+            (proj1 (List.filter_In
+                      (fun e => ThreadEvent.is_normal_dec e) ehd es)).
+          { rewrite <- H0. ss. auto. }
+          i. des. unfold proj_sumbool in *. des_ifs.
+        }
+      }
+    }
+    { right. rewrite RESERVATION. splits; auto.
+      eapply reservation_only_step_trans; eauto. }
+  Qed.
+
+  Lemma merge_steps_reservation_only_step es tid c1 c2 c3
+        (STEP0: steps es tid c1 c2)
+        (STEP1: reservation_only_step tid c2 c3)
+    :
+      (<<STEPS: steps (List.filter ThreadEvent.is_normal_dec es) tid c1 c3>>) \/
+      ((<<STEP: reservation_only_step tid c1 c3>>) /\
+       (<<RESERVATION: List.filter ThreadEvent.is_normal_dec es = []>>)).
+  Proof.
+    hexploit steps_filtering; try apply STEP0. i. des.
+    { destruct (list_match_rev (List.filter (fun e => ThreadEvent.is_normal_dec e) es)).
+      { rewrite H in *. inv STEPS. splits; auto. }
+      des. rewrite H in *. eapply steps_split in STEPS. des.
+      inv STEPS1. inv STEPS.
+      left. exploit merge_step_reservation_only_step; eauto. i. des.
+      { eapply steps_trans; eauto. }
+      { exfalso.
+        hexploit
+          (proj1 (List.filter_In
+                    (fun e => ThreadEvent.is_normal_dec e) hd_rev es)).
+        { rewrite H. eapply List.in_or_app. ss. auto. }
+        i. des. unfold proj_sumbool in *. des_ifs.
+      }
+    }
+    { right. rewrite RESERVATION. splits; auto.
+      eapply reservation_only_step_trans; eauto. }
+  Qed.
+
+  Lemma trace_step_machine_step tr e tid c1 c3
+        (STEP: Trace.configuration_step tr e tid c1 c3)
         (WF: Configuration.wf c1)
     :
-      exists c2,
-        (<<STEPS: rtc tau_machine_step c1 c2>>) /\
-        (<<STEP: machine_step e tid c2 c3>>).
+      ((<<STEPS: steps (List.filter ThreadEvent.is_normal_dec (List.map snd tr)) tid c1 c3>>) /\
+       (<<NIL: List.filter ThreadEvent.is_normal_dec (List.map snd tr) <> []>>)) \/
+      ((<<STEP: reservation_only_step tid c1 c3>>) /\
+       (<<NIL: List.filter ThreadEvent.is_normal_dec (List.map snd tr) = []>>)).
   Proof.
-    apply configuration_step_equivalent in STEP. inv STEP.
-    exploit Thread.rtc_tau_step_future; eauto.
+    inv STEP.
+    exploit Trace.steps_future; eauto.
     { eapply WF; eauto. }
     { eapply WF; eauto. }
     { eapply WF; eauto. } i. des. ss.
     clear TVIEW_FUTURE SC_FUTURE MEM_FUTURE.
-    eapply Operators_Properties.clos_rt_rt1n_iff in STEPS.
-    eapply Operators_Properties.clos_rt_rtn1_iff in STEPS.
+    eapply Trace.steps_equivalent in STEPS.
     assert (exists e2',
                (<<STEP: Thread.step pf e0 e2 e2'>>) /\
                (<<STEPS: rtc (@Thread.reserve_step _ \2/ @Thread.cancel_step _) e2' (Thread.mk _ st3 lc3 sc3 memory3)>>)).
     { eauto. }
     clear STEP0. des.
+    remember (Thread.mk _ st1 lc1 c1.(Configuration.sc) c1.(Configuration.memory)).
     ginduction STEPS.
-    { i. exploit mixed_step_step.
+    { i. subst. exploit mixed_step_step.
       { econs.
         { eauto. }
         { refl. }
@@ -231,23 +570,27 @@ Module SConfiguration.
         { eapply STEPS0. }
         { eauto. }
       }
-      i. des. esplits.
-      { refl. }
-      { replace (ThreadEvent.get_machine_event e0) with (ThreadEvent.get_machine_event e'); eauto.
-        unguard. destruct e0; des; subst; ss. }
+      i. des.
+      { ss. des_ifs.
+        { left. splits; ss. econs; [|econs 1]. eauto. }
+        { right. unfold proj_sumbool in *. des_ifs. splits; auto.
+          eapply reservation_event_reservation_only_step; eauto.
+        }
+      }
+      { right. ss. splits; auto. unfold proj_sumbool. des_ifs. }
     }
-    i. eapply rtc_implies with (R2 := @Thread.reserve_step lang \2/ @Thread.cancel_step _) in STEPS0; eauto.
+    i. subst. eapply rtc_implies with (R2 := @Thread.reserve_step lang \2/ @Thread.cancel_step _) in STEPS0; eauto.
     exploit consistent_split; try eassumption.
     { destruct (classic (e0 = ThreadEvent.failure)); auto. }
-    i. des. inv H. inv TSTEP. destruct th0'.
-    exploit Thread.rtc_tau_step_future.
-    { eapply Operators_Properties.clos_rt_rt1n_iff.
-      eapply Operators_Properties.clos_rt_rtn1_iff. eapply STEPS. }
+    i. des. destruct th0'.
+    exploit Trace.steps_future.
+    { eapply Trace.steps_equivalent. eapply STEPS. }
     { eapply WF; eauto. }
     { eapply WF; eauto. }
     { eapply WF; eauto. } i. des. ss.
+    eapply list_Forall_app in SILENT. des. inv FORALL1; ss. inv H2.
     exploit IHSTEPS; try apply STEP0; try apply RESERVESTEPS; eauto.
-    i. des. rewrite EVENT in *.
+
     exploit SConfiguration.mixed_step_step.
     { instantiate (1:=Configuration.mk
                         (IdentMap.add
@@ -272,13 +615,93 @@ Module SConfiguration.
       { erewrite IdentMap.gss. ss. }
       { econs 2; eauto. }
     }
-    i. des. erewrite IdentMap.add_add_eq in *. esplits.
-    { etrans.
-      { eapply STEPS1. }
-      { econs; [|refl]. econs; eauto. }
+    i. erewrite IdentMap.add_add_eq in *.
+    erewrite List.map_app. ss.
+    erewrite list_filter_app; eauto. ss. des_ifs.
+    { unfold proj_sumbool in Heq. des_ifs. des; ss.
+      { left. splits; ss.
+        { eapply steps_trans.
+          { eapply STEPS1. }
+          { econs 2; eauto. }
+        }
+        { ii. apply List.app_eq_nil in H. des. ss. }
+      }
+      { rewrite NIL in *. ss.
+        exploit merge_reservation_only_step_step; eauto. i. des; ss.
+        left. splits; ss. econs; eauto.
+      }
     }
-    { replace (ThreadEvent.get_machine_event e0) with (ThreadEvent.get_machine_event e'); eauto.
-      unguard. destruct e0; des; subst; ss. }
+    { erewrite List.app_nil_r in *.
+      unfold proj_sumbool in Heq. des_ifs. des; ss.
+      { eapply reservation_event_reservation_only_step in STEP0; eauto.
+        exploit merge_steps_reservation_only_step; eauto. i.
+        erewrite list_filter_idempotent in *. des; ss; eauto. }
+      { exploit merge_steps_reservation_only_step; eauto. i.
+        erewrite list_filter_idempotent in *. des; ss; eauto. }
+      { eapply reservation_event_reservation_only_step in STEP1; eauto.
+        right. splits; auto. eapply reservation_only_step_trans; eauto. }
+      { right. splits; auto. eapply reservation_only_step_trans; eauto. }
+    }
+  Qed.
+
+  Lemma list_filter_forall A P (Q R: A -> Prop) (l: list A)
+        (FORALL: List.Forall Q l)
+        (REL: forall a (SAT0: P a = true) (SAT1: Q a), R a)
+    :
+      List.Forall R (List.filter P l).
+  Proof.
+    induction l; ss. inv FORALL. des_ifs; eauto.
+  Qed.
+
+  Lemma list_map_forall A B (P: A -> Prop) (Q: B -> Prop) f (l: list A)
+        (FORALL: List.Forall P l)
+        (REL: forall a (SAT: P a), Q (f a))
+    :
+      List.Forall Q (List.map f l).
+  Proof.
+    induction l; ss. inv FORALL. eauto.
+  Qed.
+
+  Lemma multi_step_machine_step e tid c1 c3
+        (STEP: Configuration.step e tid c1 c3)
+        (WF: Configuration.wf c1)
+    :
+      exists c2,
+        (<<STEPS: rtc tau_machine_step c1 c2>>) /\
+        (<<STEP: opt_machine_step e tid c2 c3>>).
+  Proof.
+    eapply Trace.configuration_step_step in STEP. des.
+    exploit trace_step_machine_step; eauto. i. des.
+    { inv STEP0.
+      rewrite List.map_app in *.
+      rewrite list_filter_app in *. ss.
+      eapply steps_split in STEPS. des. exists c0. splits.
+      { eapply silent_steps_tau_machine_steps; eauto.
+        eapply list_filter_forall with (Q:=fun e => ThreadEvent.get_machine_event e = MachineEvent.silent); eauto.
+        eapply list_map_forall; eauto.
+      }
+      unfold proj_sumbool in *. des_ifs.
+      { inv STEPS2. inv STEPS.
+        econs 2. econs; eauto. }
+      { inv STEPS2.
+        replace (ThreadEvent.get_machine_event e0) with MachineEvent.silent; eauto.
+        unfold ThreadEvent.is_normal in *. apply not_and_or in n. des.
+        { apply NNPP in n. unfold ThreadEvent.is_reserve in *. des_ifs. }
+        { apply NNPP in n. unfold ThreadEvent.is_cancel in *. des_ifs. }
+      }
+    }
+    { eapply reservation_only_step_step in STEP.
+      exists c1. esplits; eauto.
+      replace e with (ThreadEvent.get_machine_event ThreadEvent.silent); eauto.
+      ss. inv STEP0.
+      rewrite List.map_app in NIL.
+      rewrite list_filter_app in NIL.
+      eapply List.app_eq_nil in NIL.
+      ss. unfold proj_sumbool in NIL. des. des_ifs.
+      unfold ThreadEvent.is_normal in *. apply not_and_or in n. des.
+      { apply NNPP in n. unfold ThreadEvent.is_reserve in *. des_ifs. }
+      { apply NNPP in n. unfold ThreadEvent.is_cancel in *. des_ifs. }
+    }
   Qed.
 
   Lemma machine_step_multi_step e tid c1 c3
@@ -332,7 +755,8 @@ Module SConfiguration.
       { eapply rtc_tail in AFTERSTEPS. des; clarify.
         inv AFTERSTEPS0. inv TSTEP.
         econs 2. rewrite <- EVENT0.
-        replace (IdentMap.add tid (existT _ _ st4, lc4) (Configuration.threads c1)) with (IdentMap.add tid (existT _ _ st4, lc4) (IdentMap.add tid (existT _ _ state, local) (Configuration.threads c1))).
+        replace (IdentMap.add tid (existT _ _ st4, lc4) (Configuration.threads c1)) with (IdentMap.add tid (existT _ _ st4, lc4) (IdentMap.add tid (existT _ _ state, local) (Configuration.threads c1)))
+        .
         { econs; ss.
           { eapply IdentMap.gss. }
           { eapply AFTERSTEPS. }
@@ -383,19 +807,21 @@ Module SConfiguration.
         eapply multi_step_machine_step in STEP; eauto. des.
         eapply rtc_tau_step_behavior.
         { eapply STEPS. }
-        { econs 2; eauto. }
+        { inv STEP0. econs 2; eauto. }
       }
       { eapply multi_step_machine_step in STEP; eauto. des.
         eapply rtc_tau_step_behavior.
         { eapply STEPS. }
-        { econs 3; eauto. }
+        { inv STEP0. econs 3; eauto. }
       }
       { exploit IHbehaviors.
         { eapply Configuration.step_future; eauto. } intros BEH.
         eapply multi_step_machine_step in STEP; eauto. des.
         eapply rtc_tau_step_behavior.
         { eapply STEPS. }
-        { econs 4; eauto. }
+        { inv STEP0; eauto.
+          econs 4; eauto.
+        }
       }
     }
     { clear WF. ginduction H; i.
