src/prop/Trace.v
@@ -320,6 +320,46 @@ Module Trace.
       rewrite <- steps_equivalent in STEPS.
       esplits; eauto.
   Qed.
+
+  Inductive configuration_step: forall (tr: Trace.t) (e:MachineEvent.t) (tid:Ident.t) (c1 c2:Configuration.t), Prop :=
+  | configuration_step_intro
+      lang tr e tr' pf tid c1 st1 lc1 e2 st3 lc3 sc3 memory3
+      (TID: IdentMap.find tid c1.(Configuration.threads) = Some (existT _ lang st1, lc1))
+      (STEPS: Trace.steps tr' (Thread.mk _ st1 lc1 c1.(Configuration.sc) c1.(Configuration.memory)) e2)
+      (SILENT: List.Forall (fun the => ThreadEvent.get_machine_event (snd the) = MachineEvent.silent) tr')
+      (STEP: Thread.step pf e e2 (Thread.mk _ st3 lc3 sc3 memory3))
+      (TR: tr = tr'++[(e2.(Thread.local), e)])
+      (CONSISTENT: forall (EVENT: e <> ThreadEvent.failure),
+          Thread.consistent (Thread.mk _ st3 lc3 sc3 memory3))
+    :
+      configuration_step tr (ThreadEvent.get_machine_event e) tid c1 (Configuration.mk (IdentMap.add tid (existT _ _ st3, lc3) c1.(Configuration.threads)) sc3 memory3)
+  .
+
+  Lemma step_configuration_step tr e tid c1 c2
+        (STEP: configuration_step tr e tid c1 c2)
+    :
+      Configuration.step e tid c1 c2.
+  Proof.
+    inv STEP. eapply silent_steps_tau_steps in STEPS; eauto.
+    destruct (classic (e0 = ThreadEvent.failure)).
+    { subst. ss. econs 1; eauto. }
+    { econs 2; eauto. }
+  Qed.
+
+  Lemma configuration_step_step e tid c1 c2
+        (STEP: Configuration.step e tid c1 c2)
+    :
+      exists tr,
+        (<<STEP: configuration_step tr e tid c1 c2>>).
+  Proof.
+    inv STEP.
+    { replace MachineEvent.failure with (ThreadEvent.get_machine_event ThreadEvent.failure); auto.
+      eapply tau_steps_silent_steps in STEPS. des. esplits.
+      econs; eauto. ss. }
+    { eapply tau_steps_silent_steps in STEPS. des. esplits.
+      econs; eauto. }
+  Qed.
+
 End Trace.
 
 Module ThreadTrace.
