src/prop/PromiseConsistent.v
@@ -160,6 +160,58 @@ Proof.
   apply tau_union.
 Qed.
 
+Lemma rtc_reserve_step_promise_consistent
+      lang th1 th2
+      (STEPS: rtc (@Thread.reserve_step lang) th1 th2)
+      (CONS: Local.promise_consistent th2.(Thread.local))
+      (WF1: Local.wf th1.(Thread.local) th1.(Thread.memory))
+      (SC1: Memory.closed_timemap th1.(Thread.sc) th1.(Thread.memory))
+      (MEM1: Memory.closed th1.(Thread.memory)):
+  Local.promise_consistent th1.(Thread.local).
+Proof.
+  eapply rtc_tau_step_promise_consistent; cycle 1; eauto.
+  eapply rtc_implies; [|eauto]. eapply Thread.reserve_step_tau_step.
+Qed.
+
+Lemma rtc_cancel_step_promise_consistent
+      lang th1 th2
+      (STEPS: rtc (@Thread.cancel_step lang) th1 th2)
+      (CONS: Local.promise_consistent th2.(Thread.local))
+      (WF1: Local.wf th1.(Thread.local) th1.(Thread.memory))
+      (SC1: Memory.closed_timemap th1.(Thread.sc) th1.(Thread.memory))
+      (MEM1: Memory.closed th1.(Thread.memory)):
+  Local.promise_consistent th1.(Thread.local).
+Proof.
+  eapply rtc_tau_step_promise_consistent; cycle 1; eauto.
+  eapply rtc_implies; [|eauto]. eapply Thread.cancel_step_tau_step.
+Qed.
+
+Lemma rtc_reserve_step_promise_consistent2
+      lang (th1 th2: Thread.t lang)
+      (CONS: Local.promise_consistent th1.(Thread.local))
+      (STEPS: rtc (@Thread.reserve_step lang) th1 th2)
+  :
+    Local.promise_consistent th2.(Thread.local).
+Proof.
+  ginduction STEPS; eauto.  i. eapply IHSTEPS.
+  inv H. inv STEP; inv STEP0; inv LOCAL. inv PROMISE. ss.
+  ii. erewrite Memory.add_o in PROMISE; eauto. des_ifs.
+  eapply CONS; eauto.
+Qed.
+
+Lemma rtc_cancel_step_promise_consistent2
+      lang (th1 th2: Thread.t lang)
+      (CONS: Local.promise_consistent th1.(Thread.local))
+      (STEPS: rtc (@Thread.cancel_step lang) th1 th2)
+  :
+    Local.promise_consistent th2.(Thread.local).
+Proof.
+  ginduction STEPS; eauto.  i. eapply IHSTEPS.
+  inv H. inv STEP; inv STEP0; inv LOCAL. inv PROMISE. ss.
+  ii. erewrite Memory.remove_o in PROMISE; eauto. des_ifs.
+  eapply CONS; eauto.
+Qed.
+
 Lemma consistent_promise_consistent
       lang th
       (CONS: @Thread.consistent lang th)
